src/Std/WP/Triple/SpecLemmas.lean
@@ -537,7 +537,7 @@ theorem Spec.throw_ExceptT_lift [MonadExceptOf ε m] (err : ε) (post : α → P
     Triple (MonadExceptOf.throw (ε:=ε) err : ExceptT ε' m α)
       (wp (MonadExceptOf.throw (ε:=ε) err : m (@Except.{u, u} ε' α))
         (fun r => match r with | .ok a => post a | .error e => epost.fst e) epost.snd) post epost :=
-  Triple.intro (by rw [WPMonad.wp_throw_lift_ExceptT_apply_eq]; apply WP.wp_consequence; intro r; cases r <;> rfl)
+  Triple.intro (by rw [WPMonad.wp_throw_lift_ExceptT_apply_eq]; apply WP.wp_monotone_post; intro r; cases r <;> rfl)
 
 
 @[spec]
@@ -572,7 +572,7 @@ theorem Spec.tryCatch_ExceptT_lift [MonadExceptOf ε m] (x : ExceptT ε' m α) (
     Triple (MonadExceptOf.tryCatch (ε:=ε) x h : ExceptT ε' m α)
       (wp (MonadExceptOf.tryCatch (ε:=ε) x h : m (@Except.{u, u} ε' α))
         (fun | .ok a => post a | .error e => epost.fst e) epost.snd) post epost :=
-  Triple.intro (by rw [WPMonad.wp_tryCatch_lift_ExceptT_apply_eq]; apply WP.wp_consequence; intro r; cases r <;> rfl)
+  Triple.intro (by rw [WPMonad.wp_tryCatch_lift_ExceptT_apply_eq]; apply WP.wp_monotone_post; intro r; cases r <;> rfl)
 
 
 @[spec]
